First-cut proof of correctness.

src/dafny/smart/exec.dfy
@@ -1,10 +1,15 @@
  include "./Trees2.dfy"
  include "./Helpers.dfy"
+ include "./IntTree.dfy"
+include "MerkleTrees.dfy"
 
  module Foo {
  
     import opened Trees
     import opened Helpers
+    import opened DiffTree
+    import opened MerkleTrees
+
 
     // function foo1<T>(p : seq<bit>, r : ITree<T>, b : seq<T>) : int 
     //     requires |p| == height(r) - 1
@@ -122,5 +127,173 @@
         } else {  
             restrictValuesOnChild(p, r, b);
         }   
+    }
+
+    lemma siblingsLeft(p : seq<bit>, l : seq<int>, r : ITree<int>, b : seq<int>, b': seq<int>, k : nat) 
+        /** Merkle tree. */
+        requires height(r) >= 2
+        requires |l| == |leavesIn(r)|
+        requires isMerkle2(r, l, diff)
+
+        /**  all leaves after the k leaf are zero. */
+        requires k < |leavesIn(r)|
+        requires forall i :: k < i < |l| ==> l[i] == 0
+
+        /** p is the path to k leaf in r. */
+        requires |p| == height(r) - 1
+        requires nodeAt(p, r) == leavesIn(r)[k]
+
+        requires |b| == |p|
+        /** `b` contains values at left siblings on path `p`. */
+        requires forall i :: 0 <= i < |b| ==> p[i] == 1 ==> b[i] == siblingAt(p[..i + 1], r).v
+
+        requires |b'| == |b| && forall i :: 0 <= i < |b'| ==> if p[i] == 1 then b'[i] == b[i] else b'[i] == 0 
+
+        ensures forall i :: 0 <= i < |b'| ==> b'[i] == siblingAt(p[..i + 1], r).v
+    {
+        t2(r, l, k, p);
+        // forall ( i :: 0 <= i < |b'| )
+        //     ensures b'[i] == siblingAt(p[..i + 1], r).v
+        // {
+        //     if p[i] == 
+        // }
+    }
+
+     function computeRootPathDiff(p : seq<bit>, b : seq<int>, seed: int) : int
+        requires |p| == |b|
+        decreases p
+    {
+        if |p| == 0 then 
+            seed
+        else 
+            var r := computeRootPathDiff(p[1..], b[1..], seed);
+            if p[0] == 0 then
+                diff(r, 0)
+            else 
+                diff(b[0], r)
+    }
+
+    lemma {:induction p} foo304(p : seq<bit>, b : seq<int>, seed: int) 
+        requires |b| == |p| 
+        requires forall i :: 0 <= i < |b| ==> p[i] == 0 ==> b[i] == 0
+        ensures computeRootPathDiff(p, b, seed) == computeRootPath(p, b, diff, seed)
+    {
+        if |p| == 0 {
+            //
+        } else {
+            var r := computeRootPathDiff(p[1..], b[1..], seed);
+            var r' := computeRootPath(p[1..], b[1..], diff, seed);
+            foo304(p[1..], b[1..], seed);
+            assert(r == r');
+            // HI: r == r'
+            
+            if p[0] == 0 {
+                calc {
+                    computeRootPathDiff(p, b, seed) ;
+                    ==
+                    diff(r, 0);
+                    == 
+                    diff(r', 0);
+                    == 
+                    computeRootPath(p, b, diff, seed);
+                }
+            } else {
+                //  p[0] == 1
+                calc {
+                    computeRootPathDiff(p, b, seed) ;
+                    ==
+                    diff(b[0], r);
+                    == 
+                    diff(b[0], r');
+                    == 
+                    computeRootPath(p, b, diff, seed);
+                }
+            }
+        }
+    }
+
+    lemma {:induction p} sameComputeDiffPath(p : seq<bit>, b : seq<int>, b': seq<int>, seed: int)
+        requires |b| == |p| == |b'|
+        requires forall i :: 0 <= i < |b| ==> p[i] == 1 ==> b[i] == b'[i]
+        ensures computeRootPathDiff(p, b, seed) == computeRootPathDiff(p, b', seed)
+    {
+        if |p| == 0 {
+            //
+        } else {
+            var r := computeRootPathDiff(p[1..], b[1..], seed);
+            var r' := computeRootPathDiff(p[1..], b'[1..], seed);
+            if p[0] == 0 {
+                //
+                calc {
+                    computeRootPathDiff(p, b, seed) ;
+                    ==
+                    diff(r, 0) ;
+                    == { sameComputeDiffPath(p[1..], b[1..], b'[1..], seed); }  
+                    diff(r', 0);
+                    ==
+                    computeRootPathDiff(p, b', seed);
+                }
+            } else {
+                calc {
+                    computeRootPathDiff(p, b, seed) ;
+                    ==
+                    diff(b[0], r) ;
+                    == { sameComputeDiffPath(p[1..], b[1..], b'[1..], seed); }  
+                    diff(b'[0], r');
+                    == 
+                    computeRootPathDiff(p, b', seed);
+                }
+            }
+        }
+    }
+
+    /**
+     *  Weakening of computeOnPathYieldsRootValue, requesting values on left siblings only, when
+     *  merkle tree and path is not last non-null leaf.
+     */
+     lemma {:induction p, r, b} computeOnPathYieldsRootValueDiff(p : seq<bit>, l : seq<int>, r : ITree<int>, b : seq<int>, k : nat) 
+        /** Merkle tree. */
+        requires height(r) >= 2
+        requires |l| == |leavesIn(r)|
+        requires isMerkle2(r, l, diff)
+
+        /**  all leaves after the k leaf are zero. */
+        requires k < |leavesIn(r)|
+        requires forall i :: k < i < |l| ==> l[i] == 0
+
+        /** p is the path to k leaf in r. */
+        requires |p| == height(r) - 1
+        requires nodeAt(p, r) == leavesIn(r)[k]
+
+        requires |b| == |p|
+        /** `b` contains values at left siblings on path `p`. */
+        requires forall i :: 0 <= i < |b| ==> p[i] == 1 ==> b[i] == siblingAt(p[..i + 1], r).v
+
+        ensures r.v == computeRootPathDiff(p, b, leavesIn(r)[k].v)
+
+        decreases r
+    {
+
+        //  define a new seq b' that holds default values for right siblings
+        //  and prove that pre-conditions of computeOnPathYieldsRootValue hold.
+
+        var b' : seq<int>;
+        assume( |b'| == |b| && forall i :: 0 <= i < |b| ==> if p[i] == 1 then b'[i] == b[i] else b'[i] == 0 ); 
+
+        t2(r, l, k, p);
+        assert(forall i :: 0 <= i < |p| ==> 
+            p[i] == 0 ==> siblingAt(p[..i + 1], r).v == 0);
+
+        siblingsLeft(p, l, r, b, b', k);
+        assert(forall i :: 0 <= i < |p| ==> b'[i] == siblingAt(p[..i + 1], r).v);
+
+        assert(forall i :: 0 <= i < |p| ==> p[i] == 0 ==> b'[i] == 0);
+
+        computeOnPathYieldsRootValue(p, r, b', diff, leavesIn(r)[k].v);
+        assert(computeRootPath(p, b', diff, leavesIn(r)[k].v) ==  r.v);
+        foo304(p, b', leavesIn(r)[k].v);
+        assert(computeRootPathDiff(p, b',  leavesIn(r)[k].v) == computeRootPath(p, b', diff,  leavesIn(r)[k].v));
+
+        sameComputeDiffPath(p, b, b', leavesIn(r)[k].v);
     }
  }
